src/Comparse.Parser.fsti
@@ -387,6 +387,7 @@ val bytes_length_nil: #bytes:Type0 -> {|bytes_like bytes|} -> #a:Type -> ps_a:pa
   Lemma (bytes_length ps_a [] = 0)
 
 type pre_length_bytes (bytes:Type0) {|bytes_like bytes|} (pre_length:nat -> bool) = b:bytes{pre_length (length b)}
+type pre_length_list (#bytes:Type0) {|bytes_like bytes|} (#a:Type) (ps_a:parser_serializer bytes a) (pre_length:nat -> bool) = l:list a{pre_length (bytes_length ps_a l)}
 type pre_length_seq (#bytes:Type0) {|bytes_like bytes|} (#a:Type) (ps_a:parser_serializer bytes a) (pre_length:nat -> bool) = s:Seq.seq a{pre_length (bytes_length ps_a (Seq.seq_to_list s))}
 
 
@@ -398,6 +399,16 @@ val ps_pre_length_bytes_is_valid:
   pre:bytes_compatible_pre bytes -> x:pre_length_bytes bytes pre_length ->
   Lemma ((ps_pre_length_bytes pre_length ps_length).is_valid pre x <==> pre x)
   [SMTPat ((ps_pre_length_bytes pre_length ps_length).is_valid pre x)]
+
+val ps_pre_length_list: #bytes:Type0 -> {|bytes_like bytes|} -> #a:Type -> pre_length:(nat -> bool) -> nat_parser_serializer bytes pre_length -> ps_a:parser_serializer bytes a -> parser_serializer bytes (pre_length_list ps_a pre_length)
+
+val ps_pre_length_list_is_valid:
+  #bytes:Type0 -> {|bytes_like bytes|} -> #a:Type ->
+  pre_length:(nat -> bool) -> ps_length:nat_parser_serializer bytes pre_length ->
+  ps_a:parser_serializer bytes a ->
+  pre:bytes_compatible_pre bytes -> x:pre_length_list ps_a pre_length ->
+  Lemma ((ps_pre_length_list pre_length ps_length ps_a).is_valid pre x <==> for_allP (ps_a.is_valid pre) x)
+  [SMTPat ((ps_pre_length_list pre_length ps_length ps_a).is_valid pre x)]
 
 val ps_pre_length_seq: #bytes:Type0 -> {|bytes_like bytes|} -> #a:Type -> pre_length:(nat -> bool) -> nat_parser_serializer bytes pre_length -> ps_a:parser_serializer bytes a -> parser_serializer bytes (pre_length_seq ps_a pre_length)
 
@@ -423,9 +434,11 @@ type tls_nat (r:size_range) = refined nat (in_range r)
 val ps_tls_nat: #bytes:Type0 -> {|bytes_like bytes|} -> r:size_range -> nat_parser_serializer bytes (in_range r)
 
 type tls_bytes (bytes:Type0) {|bytes_like bytes|} (r:size_range) = pre_length_bytes bytes (in_range r)
+type tls_list (bytes:Type0) {|bytes_like bytes|} (#a:Type) (ps_a:parser_serializer bytes a) (r:size_range) = pre_length_list ps_a (in_range r)
 type tls_seq (bytes:Type0) {|bytes_like bytes|} (#a:Type) (ps_a:parser_serializer bytes a) (r:size_range) = pre_length_seq ps_a (in_range r)
 
 let ps_tls_bytes (#bytes:Type0) {|bytes_like bytes|} (r:size_range): parser_serializer bytes (tls_bytes bytes r) = ps_pre_length_bytes (in_range r) (ps_tls_nat r)
+let ps_tls_list (#bytes:Type0) {|bytes_like bytes|} (#a:Type) (ps_a:parser_serializer bytes a) (r:size_range): parser_serializer bytes (tls_list bytes ps_a r) = ps_pre_length_list #bytes (in_range r) (ps_tls_nat r) ps_a
 let ps_tls_seq (#bytes:Type0) {|bytes_like bytes|} (#a:Type) (ps_a:parser_serializer bytes a) (r:size_range): parser_serializer bytes (tls_seq bytes ps_a r) = ps_pre_length_seq #bytes (in_range r) (ps_tls_nat r) ps_a
 
 
@@ -443,6 +456,9 @@ let ps_nat (#bytes:Type0) {|bytes_like bytes|}: parser_serializer bytes nat =
 let ps_bytes (#bytes:Type0) {|bytes_like bytes|}: parser_serializer bytes bytes =
   mk_trivial_isomorphism (ps_pre_length_bytes true_nat_pred ps_true_nat)
 
+let ps_list (#bytes:Type0) {|bytes_like bytes|} (#a:Type) (ps_a:parser_serializer bytes a): parser_serializer bytes (list a) =
+  mk_trivial_isomorphism (ps_pre_length_list true_nat_pred ps_true_nat ps_a)
+
 let ps_seq (#bytes:Type0) {|bytes_like bytes|} (#a:Type) (ps_a:parser_serializer bytes a): parser_serializer bytes (Seq.seq a) =
   mk_trivial_isomorphism (ps_pre_length_seq true_nat_pred ps_true_nat ps_a)
 
@@ -455,7 +471,9 @@ type quic_nat = refined nat quic_nat_pred
 val ps_quic_nat: #bytes:Type0 -> {| bytes_like bytes |} -> nat_parser_serializer bytes quic_nat_pred
 
 type quic_bytes (bytes:Type0) {|bytes_like bytes|} = pre_length_bytes bytes quic_nat_pred
+type quic_list (bytes:Type0) {|bytes_like bytes|} (#a:Type) (ps_a:parser_serializer bytes a) = pre_length_list ps_a quic_nat_pred
 type quic_seq (bytes:Type0) {|bytes_like bytes|} (#a:Type) (ps_a:parser_serializer bytes a) = pre_length_seq ps_a quic_nat_pred
 
 let ps_quic_bytes (#bytes:Type0) {|bytes_like bytes|}: parser_serializer bytes (quic_bytes bytes) = ps_pre_length_bytes quic_nat_pred ps_quic_nat
+let ps_quic_list (#bytes:Type0) {|bytes_like bytes|} (#a:Type) (ps_a:parser_serializer bytes a): parser_serializer bytes (quic_list bytes ps_a) = ps_pre_length_list #bytes quic_nat_pred ps_quic_nat ps_a
 let ps_quic_seq (#bytes:Type0) {|bytes_like bytes|} (#a:Type) (ps_a:parser_serializer bytes a): parser_serializer bytes (quic_seq bytes ps_a) = ps_pre_length_seq #bytes quic_nat_pred ps_quic_nat ps_a
